src/typ/fv.lean
@@ -1,0 +1,25 @@
+import .core
+
+namespace tts ------------------------------------------------------------------
+namespace typ ------------------------------------------------------------------
+variables {V : Type} -- Type of variable names
+variables {x x₁ x₂ : V} -- Variable names
+variables {t t₁ t₂ : typ V} -- Types
+variables {ts ts₁ ts₂ : list (typ V)} -- Lists of types
+
+variables [_root_.decidable_eq V]
+
+@[simp]
+theorem fv_not_mem_varf : x₁ ∉ fv (varf x₂) ↔ x₁ ≠ x₂ :=
+  by simp [fv]
+
+@[simp]
+theorem fv_not_mem_arr : x ∉ fv (arr t₁ t₂) ↔ x ∉ fv t₁ ∧ x ∉ fv t₂ :=
+  by simp [fv, decidable.not_or_iff_and_not]
+
+@[simp]
+theorem fv_list_append : fv_list (ts₁ ++ ts₂) = fv_list ts₁ ∪ fv_list ts₂ :=
+  by induction ts₁ with _ _ ih; [simp, simp [ih]]
+
+end /- namespace -/ typ --------------------------------------------------------
+end /- namespace -/ tts --------------------------------------------------------
