src/typ/open.lean
@@ -1,0 +1,17 @@
+import .core
+
+namespace tts ------------------------------------------------------------------
+namespace typ ------------------------------------------------------------------
+variables {i : ℕ} -- Natural numbers
+variables {V : Type} -- Type of variable names
+variables {x : V} -- Variable names
+variables {t t₁ t₂ : typ V} -- Types
+variables {ts : list (typ V)} -- Lists of types
+
+-- Opening a locally-closed type is the identity
+@[simp]
+theorem open_lc (p : lc t) : t.open ts = t :=
+  by induction t; cases p; simp [typ.open, *]
+
+end /- namespace -/ typ --------------------------------------------------------
+end /- namespace -/ tts --------------------------------------------------------
